theories/std/for_upto.v
@@ -9,32 +9,12 @@ From zebre Require Import
   options.
 
 Implicit Types δ : nat.
-Implicit Types fn : val.
-
-Definition for_upto : val :=
-  rec: "for_upto" "beg" "end" "fn" :=
-    ifnot: "end" ≤ "beg" then (
-      "fn" "beg" ;;
-      "for_upto" (#1 + "beg") "end" "fn"
-    ).
-
-Notation "'for:' i = beg 'to' _end 'begin' e 'end'" := (
-  (Val for_upto) beg _end (Lam i e)
-)(i at level 1,
-  beg, _end, e at level 200,
-  format "'[hv' for:  i  =  beg  to  _end  begin  '/  ' '[' e ']'  '/' end ']'"
-) : expr_scope.
-Notation "'for::' i = beg 'to' _end 'begin' e 'end'" := (
-  (Val for_upto) beg _end (Val (ValLam i e))
-)(i at level 1,
-  beg, _end, e at level 200,
-  format "'[hv' for::  i  =  beg  to  _end  begin  '/  ' '[' e ']'  '/' end ']'"
-) : expr_scope.
+Implicit Types body : expr.
 
 Section zebre_G.
   Context `{zebre_G : !ZebreG Σ}.
 
-  #[local] Lemma for_upto_spec_stronger beg i δ Ψ _end fn :
+  #[local] Lemma for_upto_spec_stronger beg i δ Ψ _end body :
     i = (beg + δ)%Z →
     {{{
       ▷ Ψ i δ ∗
@@ -42,53 +22,55 @@ Section zebre_G.
         ∀ i δ,
         ⌜i = (beg + δ)%Z ∧ (i < _end)%Z⌝ -∗
         Ψ i δ -∗
-        WP fn #i {{ res,
+        WP body #i {{ res,
           ⌜res = ()%V⌝ ∗
           ▷ Ψ (1 + i)%Z (S δ)
         }}
       )
     }}}
-      for_upto #i #_end fn
+      For #i #_end body
     {{{
       RET ();
       Ψ (i `max` _end)%Z (δ + Z.to_nat (_end - i))
     }}}.
   Proof.
-    iIntros "%Hi %Φ (HΨ & #Hfn) HΦ".
+    iIntros "%Hi %Φ (HΨ & #Hbody) HΦ".
     remember (Z.to_nat (_end - i)) as ϵ eqn:Hϵ.
-    iInduction ϵ as [| ϵ] "IH" forall (i δ Hi Hϵ);
-      wp_rec; wp_pures credit:"H£".
-    - assert (i `max` _end = i)%Z as -> by lia. rewrite Nat.add_0_r. iSteps.
-    - rewrite bool_decide_eq_false_2; first lia. wp_pures.
-      wp_apply (wp_wand with "(Hfn [] HΨ)") as "%res (-> & HΨ)"; first iSteps.
+    iInduction ϵ as [| ϵ] "IH" forall (i δ Hi Hϵ).
+    all: wp_for credit:"H£".
+    - rewrite decide_True; first lia.
+      assert (i `max` _end = i)%Z as -> by lia.
+      rewrite Nat.add_0_r. iSteps.
+    - rewrite decide_False; first lia.
+      wp_apply (wp_wand with "(Hbody [] HΨ)") as "%res (-> & HΨ)"; first iSteps.
       iMod (lc_fupd_elim_later with "H£ HΨ") as "HΨ".
       wp_smart_apply ("IH" with "[] [] HΨ [HΦ]"); [iSteps.. |].
       assert ((1 + i) `max` _end = i `max` _end)%Z as -> by lia. rewrite -Nat.add_succ_comm //.
   Qed.
-  Lemma for_upto_spec_strong Ψ beg _end fn :
+  Lemma for_upto_spec_strong Ψ beg _end body :
     {{{
       ▷ Ψ beg 0 ∗
       □ (
         ∀ i δ,
         ⌜i = (beg + δ)%Z ∧ (i < _end)%Z⌝ -∗
         Ψ i δ -∗
-        WP fn #i {{ res,
+        WP body #i {{ res,
           ⌜res = ()%V⌝ ∗
           ▷ Ψ (1 + i)%Z (S δ)
         }}
       )
     }}}
-      for_upto #beg #_end fn
+      For #beg #_end body
     {{{
       RET ();
       Ψ (beg `max` _end)%Z (Z.to_nat (_end - beg))
     }}}.
   Proof.
-    iIntros "%Φ (HΨ & #Hfn) HΦ".
-    wp_apply (for_upto_spec_stronger beg beg 0 with "[$HΨ $Hfn]"); first lia.
+    iIntros "%Φ (HΨ & #Hbody) HΦ".
+    wp_apply (for_upto_spec_stronger with "[$HΨ $Hbody]"); first lia.
     iSteps.
   Qed.
-  Lemma for_upto_spec Ψ beg _end fn :
+  Lemma for_upto_spec Ψ beg _end body :
     (beg ≤ _end)%Z →
     {{{
       ▷ Ψ beg 0 ∗
@@ -96,13 +78,13 @@ Section zebre_G.
         ∀ i δ,
         ⌜i = (beg + δ)%Z ∧ (i < _end)%Z⌝ -∗
         Ψ i δ -∗
-        WP fn #i {{ res,
+        WP body #i {{ res,
           ⌜res = ()%V⌝ ∗
           ▷ Ψ (1 + i)%Z (S δ)
         }}
       )
     }}}
-      for_upto #beg #_end fn
+      For #beg #_end body
     {{{
       RET ();
       Ψ _end (Z.to_nat (_end - beg))
@@ -112,37 +94,37 @@ Section zebre_G.
     wp_apply (for_upto_spec_strong Ψ with "H").
     rewrite Z.max_r //.
   Qed.
-  Lemma for_upto_spec_strong' Ψ beg _end fn :
+  Lemma for_upto_spec_strong' Ψ beg _end body :
     {{{
       ▷ Ψ beg 0 ∗
       ( [∗ list] δ ∈ seq 0 (Z.to_nat (_end - beg)),
         ∀ i,
         ⌜i = (beg + δ)%Z⌝ -∗
         Ψ i δ -∗
-        WP fn #i {{ res,
+        WP body #i {{ res,
           ⌜res = ()%V⌝ ∗
           ▷ Ψ (1 + i)%Z (S δ)
         }}
       )
     }}}
-      for_upto #beg #_end fn
+      For #beg #_end body
     {{{
       RET ();
       Ψ (beg `max` _end)%Z (Z.to_nat (_end - beg))
     }}}.
   Proof.
-    iIntros "%Φ (HΨ & Hfn) HΦ".
+    iIntros "%Φ (HΨ & Hbody) HΦ".
     match goal with |- context [big_opL bi_sep (λ _, ?Ξ') _] => set Ξ := Ξ' end.
     pose (Ψ' i δ := (
       Ψ i δ ∗
       [∗ list] ϵ ∈ seq δ (Z.to_nat (_end - beg) - δ), Ξ ϵ
     )%I).
-    wp_apply (for_upto_spec_strong Ψ' with "[HΨ Hfn]"); last iSteps.
+    wp_apply (for_upto_spec_strong Ψ' with "[HΨ Hbody]"); last iSteps.
     rewrite /Ψ' Nat.sub_0_r. iFrame. iIntros "!> %i %δ %Hi (HΨ & HΞ)".
     assert (Z.to_nat (_end - beg) - δ = S $ Z.to_nat (_end - beg) - S δ) as -> by lia.
     iSteps.
   Qed.
-  Lemma for_upto_spec' Ψ beg _end fn :
+  Lemma for_upto_spec' Ψ beg _end body :
     (beg ≤ _end)%Z →
     {{{
       ▷ Ψ beg 0 ∗
@@ -150,13 +132,13 @@ Section zebre_G.
         ∀ i,
         ⌜i = (beg + δ)%Z⌝ -∗
         Ψ i δ -∗
-        WP fn #i {{ res,
+        WP body #i {{ res,
           ⌜res = ()%V⌝ ∗
           ▷ Ψ (1 + i)%Z (S δ)
         }}
       )
     }}}
-      for_upto #beg #_end fn
+      For #beg #_end body
     {{{
       RET ();
       Ψ _end (Z.to_nat (_end - beg))
@@ -166,18 +148,18 @@ Section zebre_G.
     wp_apply (for_upto_spec_strong' Ψ with "H").
     rewrite Z.max_r //.
   Qed.
-  Lemma for_upto_spec_disentangled Ψ beg _end fn :
+  Lemma for_upto_spec_disentangled Ψ beg _end body :
     {{{
       □ (
         ∀ i δ,
         ⌜i = (beg + δ)%Z ∧ (i < _end)%Z⌝ -∗
-        WP fn #i {{ res,
+        WP body #i {{ res,
           ⌜res = ()%V⌝ ∗
           ▷ Ψ i δ
         }}
       )
     }}}
-      for_upto #beg #_end fn
+      For #beg #_end body
     {{{
       RET ();
       ( [∗ list] δ ∈ seq 0 (Z.to_nat (_end - beg)),
@@ -185,26 +167,26 @@ Section zebre_G.
       )
     }}}.
   Proof.
-    iIntros "%Φ #Hfn HΦ".
+    iIntros "%Φ #Hbody HΦ".
     pose (Ψ' (i : Z) δ := (
       [∗ list] δ' ∈ seq 0 δ, Ψ (beg + δ')%Z δ'
     )%I).
     wp_apply (for_upto_spec_strong Ψ'); last iSteps. iSplit; first iSteps. iIntros "!> %i %δ (%Hi1 & %Hi2) HΨ'".
-    wp_apply (wp_wand with "(Hfn [//])") as "%res (-> & HΨ)". iStep.
+    wp_apply (wp_wand with "(Hbody [//])") as "%res (-> & HΨ)". iStep.
     rewrite /Ψ' seq_S big_sepL_snoc Hi1. iSteps.
   Qed.
-  Lemma for_upto_spec_disentangled' Ψ beg _end fn :
+  Lemma for_upto_spec_disentangled' Ψ beg _end body :
     {{{
       ( [∗ list] δ ∈ seq 0 (Z.to_nat (_end - beg)),
         ∀ i,
         ⌜i = (beg + δ)%Z⌝ -∗
-        WP fn #i {{ res,
+        WP body #i {{ res,
           ⌜res = ()%V⌝ ∗
           ▷ Ψ i δ
         }}
       )
     }}}
-      for_upto #beg #_end fn
+      For #beg #_end body
     {{{
       RET ();
       ( [∗ list] δ ∈ seq 0 (Z.to_nat (_end - beg)),
@@ -212,36 +194,36 @@ Section zebre_G.
       )
     }}}.
   Proof.
-    iIntros "%Φ Hfn HΦ".
+    iIntros "%Φ Hbody HΦ".
     pose (Ψ' (i : Z) δ := (
       [∗ list] δ' ∈ seq 0 δ, Ψ (beg + δ')%Z δ'
     )%I).
-    wp_apply (for_upto_spec_strong' Ψ' with "[Hfn]"); last iSteps. iSplit; first iSteps.
-    iApply (big_sepL_impl with "Hfn"). iIntros "!>" (δ δ_ (-> & Hδ)%lookup_seq) "Hfn %i -> HΨ' /=".
-    wp_apply (wp_wand with "(Hfn [//])") as "%res (-> & HΨ)". iStep.
+    wp_apply (for_upto_spec_strong' Ψ' with "[Hbody]"); last iSteps. iSplit; first iSteps.
+    iApply (big_sepL_impl with "Hbody"). iIntros "!>" (δ δ_ (-> & Hδ)%lookup_seq) "Hbody %i -> HΨ' /=".
+    wp_apply (wp_wand with "(Hbody [//])") as "%res (-> & HΨ)". iStep.
     rewrite /Ψ' seq_S big_sepL_snoc. iSteps.
   Qed.
 
-  Lemma for_upto_spec_nat_strong Ψ beg _end fn :
+  Lemma for_upto_spec_nat_strong Ψ beg _end body :
     {{{
       ▷ Ψ beg 0 ∗
       □ (
         ∀ i δ,
         ⌜i = (beg + δ)%nat ∧ i < _end⌝ -∗
         Ψ i δ -∗
-        WP fn #i {{ res,
+        WP body #i {{ res,
           ⌜res = ()%V⌝ ∗
           ▷ Ψ (S i) (S δ)
         }}
       )
     }}}
-      for_upto #beg #_end fn
+      For #beg #_end body
     {{{
       RET ();
       Ψ (beg `max` _end) (_end - beg)
     }}}.
   Proof.
-    iIntros "%Φ (HΨ & #Hfn) HΦ".
+    iIntros "%Φ (HΨ & #Hbody) HΦ".
     pose Ψ' i δ :=
       Ψ (Z.to_nat i) δ.
     wp_apply (for_upto_spec_strong Ψ' with "[HΨ]").
@@ -249,7 +231,7 @@ Section zebre_G.
       rewrite -Nat2Z.inj_add Z.add_1_l -Nat2Z.inj_succ !Nat2Z.id. iSteps.
     - rewrite /Ψ' -Nat2Z.inj_max Z2Nat.inj_sub; first lia. rewrite !Nat2Z.id //.
   Qed.
-  Lemma for_upto_spec_nat Ψ beg _end fn :
+  Lemma for_upto_spec_nat Ψ beg _end body :
     beg ≤ _end →
     {{{
       ▷ Ψ beg 0 ∗
@@ -257,13 +239,13 @@ Section zebre_G.
         ∀ i δ,
         ⌜i = (beg + δ)%nat ∧ i < _end⌝ -∗
         Ψ i δ -∗
-        WP fn #i {{ res,
+        WP body #i {{ res,
           ⌜res = ()%V⌝ ∗
           ▷ Ψ (S i) (S δ)
         }}
       )
     }}}
-      for_upto #beg #_end fn
+      For #beg #_end body
     {{{
       RET ();
       Ψ _end (_end - beg)
@@ -273,35 +255,35 @@ Section zebre_G.
     wp_apply (for_upto_spec_nat_strong Ψ with "H").
     rewrite Nat.max_r //.
   Qed.
-  Lemma for_upto_spec_nat_strong' Ψ beg _end fn :
+  Lemma for_upto_spec_nat_strong' Ψ beg _end body :
     {{{
       ▷ Ψ beg 0 ∗
       ( [∗ list] δ ∈ seq 0 (_end - beg),
         ∀ i,
         ⌜i = (beg + δ)%nat⌝ -∗
         Ψ i δ -∗
-        WP fn #i {{ res,
+        WP body #i {{ res,
           ⌜res = ()%V⌝ ∗
           ▷ Ψ (S i) (S δ)
         }}
       )
     }}}
-      for_upto #beg #_end fn
+      For #beg #_end body
     {{{
       RET ();
       Ψ (beg `max` _end) (_end - beg)
     }}}.
   Proof.
-    iIntros "%Φ (HΨ & Hfn) HΦ".
+    iIntros "%Φ (HΨ & Hbody) HΦ".
     pose Ψ' i δ :=
       Ψ (Z.to_nat i) δ.
-    wp_apply (for_upto_spec_strong' Ψ' with "[HΨ Hfn]").
+    wp_apply (for_upto_spec_strong' Ψ' with "[HΨ Hbody]").
     - rewrite /Ψ' !Nat2Z.id Z2Nat.inj_sub; first lia. rewrite !Nat2Z.id. iFrame.
-      iApply (big_sepL_impl with "Hfn"). iIntros "!>" (δ δ_ (-> & Hδ)%lookup_seq) "Hfn %i -> HΨ /=".
+      iApply (big_sepL_impl with "Hbody"). iIntros "!>" (δ δ_ (-> & Hδ)%lookup_seq) "Hbody %i -> HΨ /=".
       rewrite -Nat2Z.inj_add Nat2Z.id Z.add_1_l -Nat2Z.inj_succ Nat2Z.id. iSteps.
     - rewrite /Ψ' -Nat2Z.inj_max Z2Nat.inj_sub; first lia. rewrite !Nat2Z.id //.
   Qed.
-  Lemma for_upto_spec_nat' Ψ beg _end fn :
+  Lemma for_upto_spec_nat' Ψ beg _end body :
     beg ≤ _end →
     {{{
       ▷ Ψ beg 0 ∗
@@ -309,13 +291,13 @@ Section zebre_G.
         ∀ i,
         ⌜i = (beg + δ)%nat⌝ -∗
         Ψ i δ -∗
-        WP fn #i {{ res,
+        WP body #i {{ res,
           ⌜res = ()%V⌝ ∗
           ▷ Ψ (S i) (S δ)
         }}
       )
     }}}
-      for_upto #beg #_end fn
+      For #beg #_end body
     {{{
       RET ();
       Ψ _end (_end - beg)
@@ -325,18 +307,18 @@ Section zebre_G.
     wp_apply (for_upto_spec_nat_strong' Ψ with "H").
     rewrite Nat.max_r //.
   Qed.
-  Lemma for_upto_spec_disentangled_nat Ψ beg _end fn :
+  Lemma for_upto_spec_disentangled_nat Ψ beg _end body :
     {{{
       □ (
         ∀ i δ,
         ⌜i = (beg + δ)%nat ∧ i < _end⌝ -∗
-        WP fn #i {{ res,
+        WP body #i {{ res,
           ⌜res = ()%V⌝ ∗
           ▷ Ψ i δ
         }}
       )
     }}}
-      for_upto #beg #_end fn
+      For #beg #_end body
     {{{
       RET ()%V;
       ( [∗ list] δ ∈ seq 0 (_end - beg),
@@ -344,7 +326,7 @@ Section zebre_G.
       )
     }}}.
   Proof.
-    iIntros "%Φ #Hfn HΦ".
+    iIntros "%Φ #Hbody HΦ".
     pose Ψ' i δ :=
       Ψ (Z.to_nat i) δ.
     wp_apply (for_upto_spec_disentangled Ψ').
@@ -354,18 +336,18 @@ Section zebre_G.
       setoid_rewrite <- Nat2Z.inj_add. setoid_rewrite Nat2Z.id.
       iSteps.
   Qed.
-  Lemma for_upto_spec_disentangled_nat' Ψ beg _end fn :
+  Lemma for_upto_spec_disentangled_nat' Ψ beg _end body :
     {{{
       ( [∗ list] δ ∈ seq 0 (_end - beg),
         ∀ i,
         ⌜i = (beg + δ)%nat⌝ -∗
-        WP fn #i {{ res,
+        WP body #i {{ res,
           ⌜res = ()%V⌝ ∗
           ▷ Ψ i δ
         }}
       )
     }}}
-      for_upto #beg #_end fn
+      For #beg #_end body
     {{{
       RET ();
       ( [∗ list] δ ∈ seq 0 (_end - beg),
@@ -373,30 +355,30 @@ Section zebre_G.
       )
     }}}.
   Proof.
-    iIntros "%Φ Hfn HΦ".
+    iIntros "%Φ Hbody HΦ".
     pose Ψ' i δ :=
       Ψ (Z.to_nat i) δ.
-    wp_apply (for_upto_spec_disentangled' Ψ' with "[Hfn]").
+    wp_apply (for_upto_spec_disentangled' Ψ' with "[Hbody]").
     - rewrite Z2Nat.inj_sub; first lia. rewrite !Nat2Z.id.
-      iApply (big_sepL_impl with "Hfn"). iIntros "!>" (δ δ_ (-> & Hδ)%lookup_seq) "Hfn %i -> /=".
+      iApply (big_sepL_impl with "Hbody"). iIntros "!>" (δ δ_ (-> & Hδ)%lookup_seq) "Hbody %i -> /=".
       rewrite -Nat2Z.inj_add /Ψ' Nat2Z.id. iSteps.
     - rewrite /Ψ' Z2Nat.inj_sub; first lia. rewrite !Nat2Z.id.
       setoid_rewrite <- Nat2Z.inj_add. setoid_rewrite Nat2Z.id.
       iSteps.
   Qed.
 
-  Lemma for_upto_type τ `{!iType (iProp Σ) τ} beg _end fn :
+  Lemma for_upto_type τ `{!iType (iProp Σ) τ} x beg _end body :
     {{{
-      (itype_int_range beg _end --> itype_unit)%T fn
+      (itype_int_range beg _end --> itype_unit)%T (λ: x, body)
     }}}
-      for_upto #beg #_end fn
+      for: x = #beg to #_end begin body end
     {{{
       RET (); True
     }}}.
   Proof.
-    iIntros "%Φ #Hfn HΦ".
-    wp_apply (for_upto_spec_disentangled (λ _ _, True%I)); iSteps.
+    iIntros "%Φ #Hbody HΦ".
+    wp_apply (for_upto_spec_disentangled (λ _ _, True%I)); last iSteps. iIntros "!> %i %δ %Hi".
+    wp_pure.
+    wp_apply (wp_wand with "(Hbody [])"); iSteps.
   Qed.
 End zebre_G.
-
-#[global] Opaque for_upto.
